temp/Spec.Claim.Map.fst
@@ -1,0 +1,26 @@
+module Spec.Claim.Map
+
+
+type kv (a: eqtype) (b:eqtype) = 
+  |MkKV : key: a -> value : b -> kv a b      
+
+type map (a: eqtype) (b:eqtype) = 
+	|MapCons: list (kv a b) -> map a b
+	|MapList: list a -> list b -> map a b 
+ 
+assume val size: #a: eqtype -> #b: eqtype -> map a b -> nat
+val isEmpty: #a: eqtype -> #b: eqtype -> map a b -> bool 
+val containsKey: #a: eqtype -> #b: eqtype -> map a b -> bool
+val containsValue: #a: eqtype -> #b: eqtype -> map a b -> bool
+assume val get: #a: eqtype -> #b: eqtype -> map a b -> key: a -> option b
+val put: #a: eqtype -> #b: eqtype -> map a b -> a -> b -> map a b 
+val remove: #a: eqtype -> #b: eqtype -> map a b -> map a b
+val putAll: #a: eqtype -> #b: eqtype -> map a b -> list (kv a b) -> map a b
+assume val putAll2: #a: eqtype -> #b: eqtype -> map a b -> list a -> list b -> map a b 
+val clear: #a: eqtype -> #b: eqtype -> map a b -> map a b 
+assume val keySet: #a: eqtype -> #b: eqtype -> map a b -> list a
+assume val values: #a: eqtype -> #b: eqtype -> map a b -> list b
+val equals: #a: eqtype -> #b: eqtype -> map a b -> bool
+val hashCode: #a: eqtype -> #b: eqtype -> map a b -> int
+assume val index: #a: eqtype -> #b: eqtype -> m: map a b ->index : nat {index < size m} ->  kv a b 
+
